hol-light/hol_kernelScript.sml
@@ -43,7 +43,7 @@ val _ = Hol_datatype `
 
 val _ = Hol_datatype `
   def = (* Axiomdef of hol_term
-      | *) Constdef of hol_term list => hol_term
+      | *) Constdef of (string # hol_term) list => hol_term
       | Typedef of string => hol_term => string => string`;
 
 (*
@@ -179,11 +179,28 @@ val _ = Define `
                    t <- map f t ;
                    return (h::t) od`
 
+(*
 val _ = Define `
   app f l =
     case l of
       [] => return ()
     | (h::t) => do f h ; app f t od`
+
+val _ = Define`
+  first p l =
+    case l of
+      [] => NONE
+    | (h::t) => if p h then SOME h else first p t`
+*)
+
+val _ = Define `
+  check_all_distinct ls acc msg =
+    case ls of
+      [] => return ()
+    | (h::t) =>
+      if MEM h acc then
+        failwith (msg h)
+      else check_all_distinct t (h::acc) msg`
 
 val _ = Define `
   forall p l =
@@ -379,6 +396,13 @@ val _ = Define `
          failwith ("new_constant: constant "++name++" has already been declared")
        else do ts <- get_the_term_constants ;
                set_the_term_constants ((name,ty)::ts) od od`;
+
+val _ = Define `
+  new_constants ls =
+    do cs <- get_the_term_constants ;
+       check_all_distinct (MAP FST ls) (MAP FST cs)
+         (\name. "new_constants: "++name++" appears twice or has already been declared");
+       set_the_term_constants (ls++cs) od`;
 
 (*
   let rec type_of tm =
@@ -1120,19 +1144,20 @@ val new_axiom_def = Define `
 
 val _ = Define`
   new_specification (Sequent eqs p) =
-    do vars <-
+    do eqs <-
          map (\e. do (l,r) <- dest_eq e;
                      (s,ty) <- dest_var l;
                      if ~(freesin [] r) then
-                       failwith "new_specification: a witness is not closed"
+                       failwith ("new_specification: witness for "++s++" not closed")
                      else if ~(subset (type_vars_in_term r) (tyvars ty)) then
-                       failwith "new_specification: a witness's type variables are not in its type"
-                     else return (s,ty) od) eqs ;
+                       failwith ("new_specification: type variables for "++s++" not contained in the type")
+                     else return ((s,ty),r) od) eqs ;
+       let vars = MAP FST eqs in
        if ~(freesin (MAP (UNCURRY Var) vars) p) then
-         failwith "new_specification: a free variable is not in the assumptions"
+         failwith "new_specification: specification not closed by the definitions"
        else do
-         app new_constant vars ;
-         add_def (Constdef eqs p) ;
+         new_constants vars ;
+         add_def (Constdef (MAP (\((s,ty),r). (s,r)) eqs) p) ;
          let ilist = MAP (\(s,ty). (Const s ty, Var s ty)) vars in
          let p = vsubst_aux ilist p in
          return (Sequent [] p) od od`
